---
layout: post
read_time: true
show_date: true
title:  Probability problems(1)
date:   2024-10-05 13:40:20 -0600
header-img: img/20240219/刚铎.webp
tags: [Mathematics]
author: 孙睿
mathjax: yes
catalog: true
---

Record a few probability problems that were done recently.

### EX 1 

Question source: Optiver prove it 1 [Youtube](https://www.youtube.com/watch?v=fmtscKsfMTg) 

#### Question 

Prove that 

$$ \lim_{n\rightarrow\infty} P_n = \frac{1}{2^{2n}} \sum_{i=0}^{n} \binom{n}{i}^2 = 0 
$$ 

Proof: 

Noted that $\sum_{i=0}^{n} \binom{n}{i}^2 = \binom{2n}{n}$, we have $\frac{P_{n+1}}{P_n} = \frac{2n+1}{2n+2}$. Therefore $P_n$ is a decreasing sequence with lower bound 0. So the limit holds. Claim that $P_n \leq \frac{1}{\log (2n)}$. Now prove it using induction. 

Base case: $n=1$, $P_1 = \frac{1}{2}  < \frac{1}{\log 2}$. 

Suppose that $P_n \leq \frac{1}{\log (2n)}$ holds. Then we need to show that 

$$P_{n+1} = \frac{2n+1}{2n+2} P_n \leq \frac{2n+1}{2n+2}\frac{1}{\log (2n)} \leq \frac{1}{\log (2n+2)}$$

Define $u = \frac{1}{n} \in (0,1]$, we just need to show that 

$$ f(u) = 1 + \frac{u}{u+2} - \log(1+u) \geq 0 $$ 

Noted that $f'(u) < 0$, so $f(u)$ is decreasing. Hence $f(u) \geq f(1) = \frac{4}{3} - \log 2$ is non-negative. Hence the claim holds. Therefore we have 

$$0 \leq \lim_{n\rightarrow\infty} P_n \leq \lim_{n\rightarrow\infty}\frac{1}{\log (2n)} = 0$$

#### Question 

Prove that $P_n > \frac{1}{n}$.

Proof：

It can be proved directly using induction. Try to prove it using Cauchy inequality. 

$$ n\sum_{i=0}^{n} \binom{n}{i}^2 \geq (\sum_{i=0}^{n} \binom{n}{i})^{2} = 2^{2n}$$

Hence $P_n  > \frac{1}{n}$. It is easy to check that the equality does not hold. 

### EX 2

Question source: Optiver prove it 2 [Youtube](https://www.youtube.com/watch?v=u76c4QDHXME)

#### Question 

Prove that $E_{0n} = n^{2}$

Proof:

We have $E_{i,j} = 1 + \frac{1}{2}(E_{i-1,j} + E_{i+1,j})$. Denote $a_{i} = E_{i,n}$. Then we have that 

$$
\begin{equation}
\begin{aligned}
a_0 &= 1+a_1 \\
a_1 &= 1 + \frac{1}{2}(a_2 + a_0) \\
...& \\
a_{n-1} &= 1 + \frac{1}{2}(a_{n-2} + a_{n}) \\
a_n &= 0
\end{aligned}
\end{equation}
$$

Noted that $b_n = a_n - a_{n-1} = a_{n+1} - a_n + 2 = b_{n+1} + 2$. The sequence $b_n$
is an arithmetic sequence with a common difference of -2. Then $b_n = 1-2n$. Then we have

$$
a_n - a_0 = -\sum_{k=1}^{n} (2k-1)
$$ 

Hence $E_{0n} = n^2$.

#### Question 

Calculate $E_{0,n}$ with a biased coin, whose probability of heads is $\frac{1}{3}$.

In this case, we have $E_{k,n} = 1 + \frac{2}{3}E_{k-1,n} + \frac{1}{3}E_{k+1,n}$. Similarly, we have 

$$ \frac{2}{3}b_k = \frac{2}{3}(a_{k} - a_{k-1}) = \frac{1}{3}(a_{k+1} - a_{k}) +1 $$

Hence $b_{k+1} - 3 = 2(b_k - 3) = ... = 2^{k}(b_1 - 3) = -2^{k+2}$, Then we have 

$$ a_n - a_0 = 3n - 2\sum_{i=1}^{n} 2^{i} $$ 

Hence $E_{0n} = -3n + 4(2^n - 1)$ 

### EX 3 

Question source: Optiver prove it 3 [Youtube](https://www.youtube.com/watch?v=YKE5SRXK_nI)

#### My solution

**Question**:

You and your friend take turns rolling a six-sided dice and you keep a joint running total. The player who first gets the sum to 6 or greater gets paid out the sum.

Do you want to go first or second?

**Answer**:

Go second.

**Proof**:

Define $N = \inf \{n \geq 1, \sum_{i=1}^{n}X_{i} \geq 6\}$ is the time game stops. $N_1 = \inf \{n \geq 1, \sum_{i=1}^{n}X_{i} \geq 6, n\in 2\mathbf{N} - 1 \}$ is the time when first player wins, $N_{2} = \inf \{n \geq 1, \sum_{i=1}^{n}X_{i} \geq 6, n\in 2\mathbf{N}\}$ is the time when second player wins, where $X_i$ is the result of the dice roll. We need to compare the expected value of $\sum_{i=1}^{N_1}X_i$ and $\sum_{i=1}^{N_2} X_{i}$. 

It can be shown that both $N_{1}$ and $N_{2}$ are stopping times. According to Wald's equation, we have: 

$$
\begin{equation}
\begin{aligned}
E[\sum_{i=1}^{N_1}X_i] &= E[X]E[N_1] \\
E[\sum_{i=1}^{N_2}X_i] &= E[X]E[N_2]
\end{aligned}
\end{equation}
$$

It is easily to calute $E[X] = \frac{7}{2}$. Try to calculate $E[N_i]$. 

$$
\begin{aligned}
E[N_2] &= 2*P(N=2) + 4P(N=4) + 6P(N=6) \\
P(N=k) &= P(N > k) - P(N >(k+1)) \\
&= \frac{1}{6^k} \binom{5}{k}- \frac{1}{6^{k+1}}\binom{5}{k+1}
\end{aligned}
$$ 

we have $E[N_2]$ = 72449/15552, $E[N_1]$ = 45200/15552. So the second player has more expected profit. 

We could also simulate the game to find the answer. 

```python
def roll_dice():
    
    total_count = 0
    for i in range(6):
        x = np.random.randint(1,7)
        total_count += x 

        if total_count >= 6:
            break 
    
    if i % 2 == 0:
        return (0, total_count)
    else:
        return (1, total_count)

def get_expectation(win_0,win_1): 

    N = len(win_0) + len(win_1)
    dic_0 = {}
    for i in win_0:
        if i not in dic_0:
            dic_0[i] = 1 
        else:
            dic_0[i] += 1

    dic_1 = {}
    for i in win_1:
        if i not in dic_1:
            dic_1[i] = 1 
        else:
            dic_1[i] += 1
    
    expectation_0 = 0
    for key,value in dic_0.items():
        dic_0[key] = value/N
        expectation_0 += dic_0[key]*key

    expectation_1 = 0
    for key,value in dic_1.items():
        dic_1[key] = value/N
        expectation_1 += dic_1[key]*key
    return (expectation_0, dic_0), (expectation_1, dic_1) 

from tqdm import tqdm
win_0 = []
win_1 = []
N = 100000

for i in tqdm(range(N)):
    res  = roll_dice()
    if res[0] == 0:
        win_0.append(res[1])
    else:
        win_1.append(res[1])

print(get_expectation(win_0,win_1))

((2.9000499999999994, {6: 0.21398, 8: 0.04789, 7: 0.04709, 10: 0.03255, 9: 0.04137, 11: 0.01869}), (4.6604, {8: 0.11893, 9: 0.09054, 6: 0.14704, 7: 0.14656, 11: 0.03234, 10: 0.06302}))
```